extracting recursion effect (naive version)

theories/test.v
@@ -1,8 +1,18 @@
-From Stdlib Require Import Nat Extraction PrimString.
+From Stdlib Require Import Nat List Extraction PrimString.
 
 Declare ML Module "extraction-experiments.plugin".
 
 Notation "f '$' x" := (f x) (at level 67, right associativity, only parsing).
+
+Fixpoint list_nth_option {A} (n : nat) (xs : list A) : option A :=
+  match xs with
+  | nil => None
+  | x :: xs =>
+    match n with
+    | 0 => Some x
+    | S n => list_nth_option n xs
+    end
+  end.
 
 (*******************************************************************)
 (** * Extraction for built-in datatypes. *)
@@ -63,29 +73,57 @@ Definition seq {E A B} (t : hitree E A) (u : hitree E B) : hitree E B :=
 
 Notation "t >> u" := (seq t u) (right associativity, at level 70).
 
-(** Sum of effects. *)
-Variant sumE (E1 E2 : Type -> Type) (A : Type) : Type :=
-| sumE_l (e : E1 A)
-| sumE_r (e : E2 A).
+(** Sub-effects. *)
+Class SubEffect (E F : Type -> Type) := {
+  inj_effect : forall A, E A -> F A
+}.
 
-Arguments sumE_l {E1 E2 A}.
-Arguments sumE_r {E1 E2 A}.
+Arguments inj_effect {E F _ A}.
 
-Notation "E +' F" := (sumE E F) (at level 60, right associativity).
+Notation "E '-<' F" := (SubEffect E F) (at level 60, no associativity).
+
+Definition trigger {E F A} `{E -< F} (e : E A) : hitree F A :=
+  Vis (inj_effect e).
 
 (** Print effect. *)
 Variant printE : Type -> Type :=
 | Print (s : string) : printE unit.
 
+Definition print {E} `{printE -< E} (s : string) : hitree E unit :=
+  trigger (Print s).
+
 (** Failure effect. *)
 Variant failE : Type -> Type :=
 | Fail {A} (s : string) : failE A.
+
+Definition fail {E A} `{failE -< E} (s : string) : hitree E A :=
+  trigger (Fail s).
 
 (** Iteration effect. *)
 Variant iterE (E : Type -> Type) : Type -> Type :=
 | Iter {A B} (init : A) (step : A -> hitree E (A + B)) : iterE E B.
 
 Arguments Iter {E A B}.
+
+Definition iter {E A B} `{iterE E -< E} (init : A) (step : A -> hitree E (A + B)) : hitree E B :=
+  trigger (Iter init step).
+
+(** Recursion effect. *)
+Variant recE (E : Type -> Type) : Type -> Type :=
+| MkFix {A B} (F : nat -> A -> hitree E B) (a : A) : recE E B
+| Call {A B} (x : nat) (a : A) : recE E B.
+
+Arguments MkFix {E A B}.
+Arguments Call {E A B}.
+
+Definition mkfix {E A B} `{recE E -< E} (F : nat -> A -> hitree E B) (a : A) : hitree E B :=
+  trigger (MkFix F a).
+
+Definition call {E A B} `{recE E -< E} (x : nat) (a : A) : hitree E B :=
+  trigger (Call x a).
+
+Definition fix_ {E A B} `{recE E -< E} (F : (A -> hitree E B) -> (A -> hitree E B)) (a : A) : hitree E B :=
+  mkfix (fun x a => F (call x) a) a.
 
 (*******************************************************************)
 (** * Extracting the monad. *)
@@ -102,6 +140,10 @@ Inductive fuel :=
     out of fuel in OCaml! *)
 Extract Inductive fuel => "unit" [ "()" "(fun _ -> ())" ] "(fun f0 f1 _ -> f1 ())".
 
+(** Ocaml's [Obj.magic]. *)
+Parameter ocaml_obj_magic : forall {A B}, A -> B.
+Extract Inlined Constant ocaml_obj_magic => "Obj.magic".
+
 (** The effect handler for [Print] in OCaml. *)
 Parameter ocaml_handle_Print : string -> unit.
 Extract Inlined Constant ocaml_handle_Print => "MyPlugin.Extraction.handle_Print".
@@ -109,6 +151,17 @@ Extract Inlined Constant ocaml_handle_Print => "MyPlugin.Extraction.handle_Print
 (** The effect handler for [Fail] in OCaml. *)
 Parameter ocaml_handle_Fail : forall A, string -> A.
 Extract Inlined Constant ocaml_handle_Fail => "MyPlugin.Extraction.handle_Fail".
+
+(** Entry for a recursive function. *)
+Record entry (E : Type -> Type) := mk_entry {
+  entry_dom : Type ;
+  entry_codom : Type ;
+  entry_fun : entry_dom -> hitree E entry_codom
+}.
+
+Arguments entry_dom {E}.
+Arguments entry_codom {E}.
+Arguments entry_fun {E}.
 
 (*******************************************************************)
 (** * Testing. *)
@@ -118,48 +171,63 @@ Extract Inlined Constant ocaml_handle_Fail => "MyPlugin.Extraction.handle_Fail".
 Inductive E (A : Type) : Type :=
 | E_printE (e : printE A)
 | E_failE (e : failE A)
-| E_iterE (e : iterE E A).
+| E_iterE (e : iterE E A)
+| E_recE (e : recE E A).
 
 Arguments E_printE {A}.
 Arguments E_failE {A}.
 Arguments E_iterE {A}.
+Arguments E_recE {A}.
 
-Definition print (s : string) : hitree E unit :=
-  Vis $ E_printE $ Print s.
-
-Definition fail {A} (s : string) : hitree E A :=
-  Vis $ E_failE $ Fail s.
-
-Definition iter {A B} (init : A) (step : A -> hitree E (A + B)) : hitree E B :=
-  Vis $ E_iterE $ Iter init step.
+Instance subeffect_printE : printE -< E := { inj_effect := @E_printE }.
+Instance subeffect_failE : failE -< E := { inj_effect := @E_failE }.
+Instance subeffect_iterE : iterE E -< E := { inj_effect := @E_iterE }.
+Instance subeffect_recE : recE E -< E := { inj_effect := @E_recE }.
 
 (** Run an hitree computation with effect [E]. *)
-Fixpoint ocaml_run_hitree (n : fuel) {A} (t : hitree E A) : (A -> unit) -> unit :=
-  match n with NoFuel => (fun _ => tt) | OneMoreFuel n =>
+Fixpoint ocaml_run_hitree {A} (n : fuel) (fs : list (entry E)) (t : hitree E A) : A :=
+  match n with NoFuel => ocaml_handle_Fail _ "ocaml_run_hitree: out of fuel (should not happen)" | OneMoreFuel n =>
   match t with
   (* Ret. *)
-  | Ret x => fun k => k x
+  | Ret x => x
   (* Bind. *)
-  | Bind t f => fun k => ocaml_run_hitree n t (fun x => ocaml_run_hitree n (f x) k)
+  | Bind t f =>
+    let x := ocaml_run_hitree n fs t in
+    ocaml_run_hitree n fs (f x)
   (* Print effect. *)
   | Vis (E_printE e) =>
     match e with
-    | Print s => fun k => k $ ocaml_handle_Print s
+    | Print s => ocaml_handle_Print s
     end
   (* Failure effect. *)
   | Vis (E_failE e) =>
     match e with
-    | Fail s => fun k => k (ocaml_handle_Fail _ s)
+    | Fail s => ocaml_handle_Fail _ s
     end
   (* Iteration effect. *)
   | Vis (E_iterE e) =>
     match e with
-    | Iter init step => fun k =>
-      ocaml_run_hitree n (step init) (fun ab =>
-        match ab with
-        | inl a => ocaml_run_hitree n (Vis $ E_iterE $ Iter a step) k
-        | inr b => k b
-        end)
+    | Iter init step =>
+      let ab := ocaml_run_hitree n fs (step init) in
+      match ab with
+      | inl a => ocaml_run_hitree n fs (Vis $ E_iterE $ Iter a step)
+      | inr b => b
+      end
+    end
+  (* Recursion effect. *)
+  | Vis (E_recE e) =>
+    match e with
+    (* MkFix: add the function to the environment and run the body. *)
+    | MkFix F a =>
+      let x := List.length fs in
+      let e := mk_entry E _ _ (F x) in
+      ocaml_run_hitree n (fs ++ (e :: nil)) (F x a)
+    (* Call: Lookup the function in the environment. *)
+    | Call x a =>
+      match list_nth_option x fs with
+      | Some e => ocaml_run_hitree n fs (ocaml_obj_magic $ entry_fun e $ ocaml_obj_magic a)
+      | None => ocaml_handle_Fail _ "In ocaml_run_hitree: [Call] got an unbound function."
+      end
     end
   end
   end.
@@ -173,7 +241,14 @@ Definition for_ (start stop : nat) (body : nat -> hitree E unit) : hitree E unit
 Definition prg : hitree E unit :=
   for_ 1 5 (fun _ => print "hello") >> print "done".
 
+Definition prg_rec : hitree E unit :=
+  let loop := fix_ $ fun loop i =>
+    if Nat.ltb i 5 then print "hello" >> loop (i + 1)
+    else Ret tt
+  in
+  loop 1.
+
 Definition test : unit :=
-  ocaml_run_hitree NoFuel prg (fun _ => tt).
+  ocaml_run_hitree NoFuel nil prg_rec.
 
 Test test.
